Main.lean
@@ -1,36 +1,111 @@
 import FraudProof.DataStructures.Hash
+import FraudProof.DataStructures.BTree
+import FraudProof.DataStructures.MTree
 
 import Batteries.Lean.IO.Process -- easy run process
 
+import Mathlib.Control.Combinators -- mapM and stuff
+
 ------------------------------------------------------------
--- Absolute path to python hash function.
-def python : String
-  := "/home/mceresa/Research/WIP/LeanPOC/FraudProof/PY/venv/bin/python"
-def pyHash : String
-  := "/home/mceresa/Research/WIP/LeanPOC/FraudProof/PY/hashing.py"
+-- Relative path to python hash function.
+-- def python : String
+--   := "/home/mceresa/Research/WIP/LeanPOC/FraudProof/PY/venv/bin/python"
+
+section PythonRelPath
+  open System
+  variable (projectRoot : System.FilePath)
+  def relPydir : System.FilePath
+    := projectRoot.join $ mkFilePath ["PY"]
+
+  def relPython : System.FilePath
+    := (relPydir projectRoot).join $ mkFilePath ["venv","bin","python"]
+
+  def relPyHash : System.FilePath
+    := (relPydir projectRoot).join $ mkFilePath ["hashing.py"]
+end PythonRelPath
+
+def pythonFileP : IO System.FilePath := relPython <$> IO.currentDir
+def hashFileP : IO System.FilePath := relPyHash <$> IO.currentDir
 
 ------------------------------------------------------------
 -- Running pyHash script
 def externalHashing' (str : String) : IO (Option String) :=
-  IO.Process.runCmdWithInput' python (Array.mkArray2 pyHash str) >>=
-  fun res => return if res.stderr != "" then  none else some res.stdout
+  do
+   let python <- pythonFileP
+   let pyHash <- hashFileP
+   let res <- IO.Process.runCmdWithInput' python.toString (Array.mkArray2 pyHash.toString str)
+   if res.stderr != ""
+     then return none
+     else return (some res.stdout)
 
 def externalHashing (str : String) : IO String :=
-  IO.Process.runCmdWithInput python (Array.mkArray2 pyHash str)
+  do
+   let python <- pythonFileP
+   let pyHash <- hashFileP
+   IO.Process.runCmdWithInput python.toString (Array.mkArray2 pyHash.toString str)
 
+--------------------
+-- Hash instances (flagged as unsafe)
+unsafe instance ecck : Hash String String where
+  mhash str := match unsafeIO $ externalHashing str with
+               | .error _ => ""
+               | .ok h => h
+
+-- comb
 def combHashing (str1 str2 : String) : IO String :=
-  -- str1 ⊕ str2 = H(str1 ++ str2)
   externalHashing (str1.append str2)
 
+unsafe def unsafeExtComb (str1 str2 : String) : String
+  := match unsafeIO (combHashing str1 str2) with
+    | .error _ => ""
+    | .ok hash => hash
 
+unsafe instance ecckMagma : HashMagma String where
+  comb := unsafeExtComb
+
+------------------------------------------------------------
+-- * Laws
+-- We only need laws to prove theorems.
+--
+-- All laws are assumed. Outside this work.
+-- unsafe instance collfree : CollResistant String String where
+--   noCollisions := sorry
+-- unsafe instance magmaLaw : SLawFulHash String where
+--   neqLeft := sorry
+--   neqRight := sorry
+------------------------------------------------------------
+
+------------------------------------------------------------
+-- * Small Demo with elements
+-- .
+-- Some elements, we can IO them.
+def elements : List String := ["esto", "es", "una", "demo"]
+
+unsafe def elemsHashes : List String := elements.map ecck.mhash
+unsafe def elemsTree : BTree String :=
+  match elemsHashes.fromList with
+    | none => sorry -- it's unsafe, I don't case about stuff anymore.
+    | some t => t
+
+-- Get Merkle Tree
+unsafe def elemsMTree : MTree String := hash_BTree elemsTree
 ------------------------------------------------------------
 
 ------------------------------------------------------------
 -- Main entry point.
 def main : IO Unit :=
   do
-    let enc <- externalHashing "hasheame"
-    IO.println "Hello! This is goint to be a simple demo of our humble piece of software"
-    IO.println s!"Hashed:{enc}"
-
+    IO.println "Hello Human?"
+    IO.println "This s a simple demo of our humble piece of software"
+    IO.println s!"Elements of the tree :{elements}"
+    let encs <- Monad.mapM externalHashing elements
+    IO.println s!"Hashed elements:{encs}"
+    let btree := encs.fromList
+    IO.println "Generated a balanced tree."
+    match btree with
+      | none => IO.println "empty tree?"
+      | some t => do
+                    let mt <- hashM externalHashing combHashing t
+                    IO.println s!"And presents the following MTree root hash {mt.hash}"
+    -- let enc <- externalHashing "Testing hashing function!"
 ------------------------------------------------------------
